\begin{bmatrix}
f(n) \\ f(n+1)
\end{bmatrix}
=
\begin{bmatrix}
0 & 1 \\ b & a
\end{bmatrix}
\times
\begin{bmatrix}
f(n-1) \\ f(n)
\end{bmatrix}
---
\begin{bmatrix}
f(n) \\ f(n+1)
\end{bmatrix}
=
\begin{bmatrix}
0 & 1 \\ b & a
\end{bmatrix}
\times
\begin{bmatrix}
f(n-1) \\ f(n)
\end{bmatrix}
=
\begin{bmatrix}
0 & 1 \\ b & a
\end{bmatrix}
\times
\begin{bmatrix}
0 & 1 \\ b & a
\end{bmatrix}
\times
\begin{bmatrix}
f(n-2) \\ f(n-1)
\end{bmatrix}
=
\begin{bmatrix}
0 & 1 \\ b & a
\end{bmatrix}
\times
\ldots
\times
\begin{bmatrix}
0 & 1 \\ b & a
\end{bmatrix}
\times
\begin{bmatrix}
\alpha \\ \beta
\end{bmatrix}
---
C(n) = \sum_{i=0}^{\log n} \mathcal{O}\left( (2^{i})^{k} \right) = \mathcal{O}\left( 2^{k \log n}\right) = \mathcal{O} \left( n^{k} \right)
---
x^{n} =
\begin{cases}
 & (x^2)^{\frac{n}{2}}, \text{ if } x \text{ is even } \\
 &x(x^2)^{\frac{n-1}{2}}, \text{ if } x \text{ is odd } \\
\end{cases}
---